ref counting

disk-betree/ImplModelCache.i.dfy
@@ -80,6 +80,7 @@ module ImplModelCache {
   {
     && s.Ready?
     && IndirectionTableModel.Inv(s.ephemeralIndirectionTable)
+    && IndirectionTableModel.TrackingGarbage(s.ephemeralIndirectionTable)
     && (forall loc |
         loc in IIndirectionTable(s.ephemeralIndirectionTable).locs.Values :: 
           BC.ValidLocationForNode(loc))
@@ -88,6 +89,15 @@ module ImplModelCache {
     && ImplModelBlockAllocator.Inv(s.blockAllocator)
     && BC.AllLocationsForDifferentRefsDontOverlap(
         IIndirectionTable(s.ephemeralIndirectionTable))
+  }
+
+  predicate ChildrenConditions(k: Constants, s: Variables, succs: Option<seq<BT.G.Reference>>)
+  requires s.Ready?
+  {
+    succs.Some? ==> (
+      && |succs.value| <= MaxNumChildren()
+      && IndirectionTableModel.SuccsValid(succs.value, s.ephemeralIndirectionTable.graph)
+    )
   }
 
   lemma lemmaIndirectionTableLocIndexValid(k: Constants, s: Variables, ref: BT.G.Reference)
@@ -117,6 +127,7 @@ module ImplModelCache {
   function {:opaque} writeBookkeeping(k: Constants, s: Variables, ref: BT.G.Reference, children: Option<seq<BT.G.Reference>>)
   : (s': Variables)
   requires WriteAllocConditions(k, s)
+  requires ChildrenConditions(k, s, children)
   ensures s'.Ready?
   ensures s'.cache == s.cache
   ensures WriteAllocConditions(k, s')
@@ -143,6 +154,7 @@ module ImplModelCache {
   function {:opaque} allocBookkeeping(k: Constants, s: Variables, children: Option<seq<BT.G.Reference>>)
   : (p: (Variables, Option<Reference>))
   requires WriteAllocConditions(k, s)
+  requires ChildrenConditions(k, s, children)
 
   ensures var (s', id) := p;
     && s'.Ready?
@@ -164,6 +176,7 @@ module ImplModelCache {
   function writeWithNode(k: Constants, s: Variables, ref: BT.G.Reference, node: Node)
   : (s': Variables)
   requires WriteAllocConditions(k, s)
+  requires ChildrenConditions(k, s, node.children)
   ensures WriteAllocConditions(k, s')
   {
     lemmaIndirectionTableLocIndexValid(k, s, ref);
@@ -188,6 +201,7 @@ module ImplModelCache {
   function allocWithNode(k: Constants, s: Variables, node: Node)
   : (p: (Variables, Option<Reference>))
   requires WriteAllocConditions(k, s)
+  requires ChildrenConditions(k, s, node.children)
   ensures var (s', id) := p;
       WriteAllocConditions(k, s')
   {
@@ -343,6 +357,7 @@ module ImplModelCache {
 
   lemma writeBookkeepingBitmapCorrect(k: Constants, s: Variables, ref: BT.G.Reference, children: Option<seq<BT.G.Reference>>)
   requires WriteAllocConditions(k, s)
+  requires ChildrenConditions(k, s, children)
   ensures var s' := writeBookkeeping(k, s, ref, children);
     && WriteAllocConditions(k, s')
   {
@@ -476,4 +491,94 @@ module ImplModelCache {
   requires ref in s.cache
   ensures getFreeRef2(s, avoid) != Some(ref)
 
+  lemma lemmaChildrenConditionsOfNode(
+      k: Constants, s: Variables, ref: BT.G.Reference)
+  requires s.Ready?
+  requires Inv(k, s)
+  requires ref in s.cache
+  requires ref in s.ephemeralIndirectionTable.graph
+  ensures ChildrenConditions(k, s, s.cache[ref].children)
+  {
+    if s.cache[ref].children.Some? {
+      forall r | r in s.cache[ref].children.value
+      ensures r in s.ephemeralIndirectionTable.graph
+      {
+        // Trigger the forall in CacheConsistentWithSuccessors
+        assert r in BT.G.Successors(INode(s.cache[ref]));
+        assert r in s.ephemeralIndirectionTable.graph[ref];
+      }
+    }
+  }
+
+  lemma lemmaChildrenConditionsSingleOfAllocBookkeeping(
+      k: Constants, s: Variables, children: Option<seq<BT.G.Reference>>)
+  requires WriteAllocConditions(k, s)
+  requires ChildrenConditions(k, s, children)
+  ensures var (s1, newref) := allocBookkeeping(k, s, children);
+    newref.Some? ==> ChildrenConditions(k, s1, Some([newref.value]))
+  {
+    reveal_allocBookkeeping();
+    reveal_writeBookkeeping();
+    //assert newref.value in s1.ephemeralIndirectionTable.graph;
+  }
+
+  lemma lemmaChildrenConditionsUpdateOfAllocBookkeeping(
+      k: Constants, s: Variables, children: Option<seq<BT.G.Reference>>,
+          children1: seq<BT.G.Reference>, i: int)
+  requires WriteAllocConditions(k, s)
+  requires ChildrenConditions(k, s, children)
+  requires ChildrenConditions(k, s, Some(children1))
+  requires 0 <= i < |children1|
+  ensures var (s1, newref) := allocBookkeeping(k, s, children);
+    newref.Some? ==> ChildrenConditions(k, s1, Some(children1[i := newref.value]))
+  {
+    reveal_allocBookkeeping();
+    reveal_writeBookkeeping();
+  }
+
+  lemma lemmaChildrenConditionsPreservedWriteBookkeeping(
+      k: Constants, s: Variables, ref: BT.G.Reference, children: Option<seq<BT.G.Reference>>,
+      children1: Option<seq<BT.G.Reference>>)
+  requires WriteAllocConditions(k, s)
+  requires ChildrenConditions(k, s, children)
+  requires ChildrenConditions(k, s, children1)
+  ensures var s1 := writeBookkeeping(k, s, ref, children);
+    ChildrenConditions(k, s1, children1)
+  {
+    reveal_writeBookkeeping();
+  }
+
+  lemma lemmaChildrenConditionsOfReplace1With2(
+      k: Constants, s: Variables,
+      children: seq<BT.G.Reference>,
+      i: int, a: BT.G.Reference, b: BT.G.Reference)
+  requires s.Ready?
+  requires ChildrenConditions(k, s, Some(children))
+  requires a in s.ephemeralIndirectionTable.graph
+  requires b in s.ephemeralIndirectionTable.graph
+  requires 0 <= i < |children|
+  requires |children| < MaxNumChildren()
+  ensures ChildrenConditions(k, s, Some(replace1with2(children, a, b, i)))
+  {
+    reveal_replace1with2();
+  }
+
+  lemma lemmaRefInGraphOfWriteBookkeeping(k: Constants, s: Variables, ref: BT.G.Reference, children: Option<seq<BT.G.Reference>>)
+  requires WriteAllocConditions(k, s)
+  requires ChildrenConditions(k, s, children)
+  ensures var s1 := writeBookkeeping(k, s, ref, children);
+    ref in s1.ephemeralIndirectionTable.graph
+  {
+    reveal_writeBookkeeping();
+  }
+
+  lemma lemmaRefInGraphPreservedWriteBookkeeping(k: Constants, s: Variables, ref: BT.G.Reference, children: Option<seq<BT.G.Reference>>, ref2: BT.G.Reference)
+  requires WriteAllocConditions(k, s)
+  requires ChildrenConditions(k, s, children)
+  requires ref2 in s.ephemeralIndirectionTable.graph
+  ensures var s1 := writeBookkeeping(k, s, ref, children);
+    ref2 in s1.ephemeralIndirectionTable.graph
+  {
+    reveal_writeBookkeeping();
+  }
 }
