lib/SetBijectivity.i.dfy
@@ -1,7 +1,7 @@
 
 
 module SetBijectivity {
-  lemma BijectivityImpliesEqualCardinality<A, B>(setA: set<A>, setB: set<B>, relation: set<(A, B)>)
+  lemma BijectivityImpliesEqualCardinality<A, B>(setA: set<A>, setB: set<B>, relation: iset<(A, B)>)
     requires forall a :: a in setA ==> exists b :: b in setB && (a, b) in relation
     requires forall a1, a2, b :: a1 in setA && a2 in setA && b in setB && (a1, b) in relation && (a2, b) in relation ==> a1 == a2
     requires forall b :: b in setB ==> exists a :: a in setA && (a, b) in relation
